fv/lean/Ragu/Circuits/Point/Negate.lean
@@ -1,0 +1,43 @@
+import Clean.Circuit
+import Clean.Utils.Primes
+import Ragu.Circuits.Element.AllocSquare
+import Ragu.Circuits.Element.Mul
+import Ragu.Circuits.Element.Square
+import Ragu.Circuits.Element.DivNonzero
+import Ragu.Circuits.Point.Spec
+
+namespace Ragu.Circuits.Point.Negate
+variable {p : ℕ} [Fact p.Prime]
+
+def main (input : Var Spec.Point (F p)) : Circuit (F p) (Var Spec.Point (F p)) := do
+  let ⟨x, y⟩ := input
+  return ⟨x, -y⟩
+
+def Assumptions (curveParams : Spec.CurveParams (F p)) (input : Spec.Point (F p)) :=
+  input.isOnCurve curveParams
+
+def Spec (curveParams : Spec.CurveParams (F p)) (input : Spec.Point (F p)) (output : Spec.Point (F p)) :=
+  output = Spec.Point.negate input ∧ output.isOnCurve curveParams
+
+instance elaborated : ElaboratedCircuit (F p) Spec.Point Spec.Point where
+  main
+  localLength _ := 0
+
+theorem soundness (curveParams : Spec.CurveParams (F p)) : Soundness (F p) elaborated (Assumptions curveParams) (Spec curveParams) := by
+  circuit_proof_start
+  simp_all only [Spec.Point.isOnCurve, id_eq, Spec.Point.negate, even_two, Even.neg_pow, and_self]
+
+
+theorem completeness (curveParams : Spec.CurveParams (F p)) : Completeness (F p) elaborated (Assumptions curveParams) := by
+  sorry
+
+def circuit (curveParams : Spec.CurveParams (F p)) : FormalCircuit (F p) Spec.Point Spec.Point :=
+  {
+    elaborated with
+    Assumptions := Assumptions curveParams,
+    Spec := Spec curveParams,
+    soundness := soundness curveParams,
+    completeness := completeness curveParams
+  }
+
+end Ragu.Circuits.Point.Negate
